Coq/Coq33.v
@@ -1,0 +1,10 @@
+(*
+  Exercises for <Software Foundations> V2 CH9.
+  Author : Brethland, Early 2020.
+*)
+
+Set Warnings "-notation-overridden,-parsing".
+Require Import Strings.String.
+Add LoadPath "C:\Users\ycy12\Documents\Workspace\LEARNING-STUFF\Coq".
+Load Coq31.
+
